LTT_PLTT.v
@@ -34,13 +34,9 @@ Definition memory_wf (Is : list Component.interface) (mem : Memory.data) :=
     exists Cmem, M.MapsTo C Cmem mem.
 
 Theorem option_simulation:
-  forall split s C d mem regs pc s' ps Is E t,
-    let G := LTT.mkGlobalEnv Is E in
+  forall split s C d mem regs pc s' ps Is E EWF t,
+    let G := LTT.mkGlobalEnv Is E EWF in
     s = (C,d,mem,regs,pc) ->
-
-    (* Global environment well-formedness *)
-    (* - entrypoints exist for each declared component *)
-    LTT.global_env_wf G ->
 
     (* Memory well-formedness *)
     (* - each declared component has its own memory *)
@@ -53,18 +49,16 @@ Theorem option_simulation:
     (* Simulation argument *)
     (t = E0 /\ match_states split s' ps)
     \/
-    (forall E',
+    (forall E' E'WF SplitWF,
         (* Entrypoints preservation *)
         PLTT.maps_match_on split E E' ->
-        (* Global environment well-formedness *)
-        let G' := PLTT.mkGlobalEnv Is E' split in
-        PLTT.global_env_wf G' ->
+        let G' := PLTT.mkGlobalEnv Is E' split E'WF SplitWF in
         (* Simulation step *)
         exists ps',
           PLTT.step G' ps t ps' /\ match_states split s' ps').
 Proof.
-  intros split s C d mem regs pc s' ps Is E t.
-  intros G Hstate HGwf HmemWF Hstates_match Hstep.
+  intros split s C d mem regs pc s' ps Is E EWF t.
+  intros G Hstate HmemWF Hstates_match Hstep.
 
   inversion Hstates_match as [ C0 ? ? ? ? ? ? Hcontrol Hpstack Hmem |
                                C0 ? ? ? ? ? ? Hcontrol Hpstack Hmem ];
@@ -78,190 +72,76 @@ Proof.
 
     (* prove context epsilon steps by staying still *)
     try (left; split; 
-         [ reflexivity
-         | apply context_control;
-           try assumption;
-           try reflexivity;
-           try apply Hmem]).
+         [ | apply context_control ];
+         auto);
 
-  (* program epsilon steps *)
-  - right.
-    intros E' HE'WF G' HG'WF.
-    eexists. split.
-    (* step *)
-    + destruct (PLTT.split_wellformed G' HG'WF C1 Hcontrol)
-        as [C1I [C1_in_Is C1I_name]].
-      destruct (HmemWF C1I C1 C1_in_Is C1I_name) as [C1mem HC1mem].
-      eapply PLTT.Program_Epsilon.
-      * apply HC1mem.
-      * apply HC1mem.
-      * simpl. unfold PLTT.maps_match_on.
-        intros. split; intro; apply HE'WF; assumption.
-      * simpl. rewrite H2 in H.
-        inversion H.
-        rewrite H3 in Hstep.
-        rewrite H4 in Hstep.
-        rewrite H5 in Hstep.
-        rewrite H6 in Hstep.
-        rewrite H7 in Hstep.
-        eapply Hstep.
-      * apply Hmem. assumption.
-        rewrite H2 in H.
-        inversion H.
-        rewrite <- H3. assumption.
-      * eassumption.
-    (* states match *)
-    + simpl. rewrite H2 in H.
-      inversion H.
-      rewrite <- H7.
-      apply program_control.
-      rewrite <- H3. assumption.
-      reflexivity.
-      simpl. unfold PLTT.maps_match_on.
-      intros. split; intro; assumption.
+    (* prove program epsilon steps *)
+    try (right;
+         intros E' HE'WF SplitWF HEE'match;
+         intros G';
+         eexists; split;
+         [ (* step *)
+           destruct (PLTT.split_wellformed G' C1 Hcontrol)
+             as [C1I [C1_in_Is C1I_name]];
+           destruct (HmemWF C1I C1 C1_in_Is C1I_name)
+             as [C1mem HC1mem];
+           eapply PLTT.Program_Epsilon;
+           [ apply HC1mem
+           | apply HC1mem
+           | simpl; unfold PLTT.maps_match_on;
+             split; intro; apply HEE'match; assumption
+           | simpl;
+             match goal with
+             | Heq_state : (_, _, _, _, _) = (C, _, _, _, _)
+               |- _ =>
+               inversion Heq_state
+             end;
+             match goal with
+             | Heq_C : _ = C,
+               Heq_d : _ = d,
+               Heq_mem : _ = mem,
+               Heq_regs : _ = regs,
+               Heq_pc : _ = pc
+               |- _ =>
+               try (rewrite Heq_pc in Hstep);
+               rewrite Heq_C, Heq_d, Heq_mem, Heq_regs in Hstep
+             end;
+             apply Hstep
+           | apply Hmem;
+             [ assumption
+             | match goal with
+               | Heq_state : (_, _, _, _, _) = (C, _, _, _, _)
+                 |- _ =>
+                 inversion Heq_state
+               end;
+               match goal with
+               | Heq_C : _ = C
+                 |- _ =>
+                 rewrite <- Heq_C; auto
+               end
+             ]
+           | eassumption ]
 
-  - right.
-    intros E' HE'WF G' HG'WF.
-    eexists. split.
-    (* step *)
-    + destruct (PLTT.split_wellformed G' HG'WF C1 Hcontrol)
-        as [C1I [C1_in_Is C1I_name]].
-      destruct (HmemWF C1I C1 C1_in_Is C1I_name) as [C1mem HC1mem].
-      eapply PLTT.Program_Epsilon.
-      * apply HC1mem.
-      * apply HC1mem.
-      * simpl. unfold PLTT.maps_match_on.
-        intros. split; intro; apply HE'WF; assumption.
-      * simpl. rewrite H3 in H.
-        inversion H.
-        rewrite H2 in Hstep.
-        rewrite H4 in Hstep.
-        rewrite H5 in Hstep.
-        rewrite H6 in Hstep.
-        rewrite H7 in Hstep.
-        eapply Hstep.
-      * apply Hmem. assumption.
-        rewrite H3 in H.
-        inversion H.
-        rewrite <- H2. assumption.
-      * eassumption.
-    (* states match *)
-    + simpl. rewrite H3 in H.
-      inversion H.
-      rewrite <- H7.
-      apply program_control.
-      rewrite <- H2. assumption.
-      reflexivity.
-      simpl. unfold PLTT.maps_match_on.
-      intros. split; intro; assumption.
+         | (* states match *)
+           simpl;
+           match goal with
+           | Heq_state : (_, _, _, _, _) = (C, _, _, _, _)
+             |- _ =>
+             inversion Heq_state
+           end;
+           match goal with
+           | Heq_C : _ = C,
+             Heq_pc : _ = pc
+             |- _ =>
+             try (rewrite <- Heq_pc); apply program_control;
+             [ rewrite <- Heq_C; auto
+             | reflexivity
+             | simpl; unfold PLTT.maps_match_on;
+               intros; split; intro; assumption ]
+           end ]).
 
-  - right.
-    intros E' HE'WF G' HG'WF.
-    eexists. split.
-    (* step *)
-    + destruct (PLTT.split_wellformed G' HG'WF C1 Hcontrol)
-        as [C1I [C1_in_Is C1I_name]].
-      destruct (HmemWF C1I C1 C1_in_Is C1I_name) as [C1mem HC1mem].
-      eapply PLTT.Program_Epsilon.
-      * apply HC1mem.
-      * apply HC1mem.
-      * simpl. unfold PLTT.maps_match_on.
-        intros. split; intro; apply HE'WF; assumption.
-      * simpl. rewrite H3 in H.
-        inversion H.
-        rewrite H2 in Hstep.
-        rewrite H4 in Hstep.
-        rewrite H5 in Hstep.
-        rewrite H6 in Hstep.
-        rewrite H7 in Hstep.
-        eapply Hstep.
-      * apply Hmem. assumption.
-        rewrite H3 in H.
-        inversion H.
-        rewrite <- H2. assumption.
-      * eassumption.
-    (* states match *)
-    + simpl. rewrite H3 in H.
-      inversion H.
-      rewrite <- H7.
-      apply program_control.
-      rewrite <- H2. assumption.
-      reflexivity.
-      simpl. unfold PLTT.maps_match_on.
-      intros. split; intro; assumption.
-
-  - right.
-    intros E' HE'WF G' HG'WF.
-    eexists. split.
-    (* step *)
-    + destruct (PLTT.split_wellformed G' HG'WF C1 Hcontrol)
-        as [C1I [C1_in_Is C1I_name]].
-      destruct (HmemWF C1I C1 C1_in_Is C1I_name) as [C1mem HC1mem].
-      eapply PLTT.Program_Epsilon.
-      * apply HC1mem.
-      * apply HC1mem.
-      * simpl. unfold PLTT.maps_match_on.
-        intros. split; intro; apply HE'WF; assumption.
-      * simpl. rewrite H5 in H.
-        inversion H.
-        rewrite H2 in Hstep.
-        rewrite H3 in Hstep.
-        rewrite H4 in Hstep.
-        rewrite H6 in Hstep.
-        rewrite H7 in Hstep.
-        eapply Hstep.
-      * apply Hmem. assumption.
-        rewrite H5 in H.
-        inversion H.
-        rewrite <- H2. assumption.
-      * eassumption.
-    (* states match *)
-    + simpl. rewrite H5 in H.
-      inversion H.
-      rewrite <- H7.
-      apply program_control.
-      rewrite <- H2. assumption.
-      reflexivity.
-      simpl. unfold PLTT.maps_match_on.
-      intros. split; intro; assumption.
-
-  - right.
-    intros E' HE'WF G' HG'WF.
-    eexists. split.
-    (* step *)
-    + destruct (PLTT.split_wellformed G' HG'WF C1 Hcontrol)
-        as [C1I [C1_in_Is C1I_name]].
-      destruct (HmemWF C1I C1 C1_in_Is C1I_name) as [C1mem HC1mem].
-      eapply PLTT.Program_Epsilon.
-      * apply HC1mem.
-      * apply HC1mem.
-      * simpl. unfold PLTT.maps_match_on.
-        intros. split; intro; apply HE'WF; assumption.
-      * simpl. rewrite H5 in H.
-        inversion H.
-        rewrite H2 in Hstep.
-        rewrite H4 in Hstep.
-        rewrite H6 in Hstep.
-        rewrite H7 in Hstep.
-        rewrite H8 in Hstep.
-        eapply Hstep.
-      * apply Hmem. assumption.
-        rewrite H5 in H.
-        inversion H.
-        rewrite <- H2. assumption.
-      * eassumption.
-    (* states match *)
-    + simpl. rewrite H5 in H.
-      inversion H.
-      rewrite <- H7.
-      apply program_control.
-      rewrite <- H2. assumption.
-      reflexivity.
-      simpl. unfold PLTT.maps_match_on.
-      intros. split; intro; assumption.
-
-  (* store *)
-  - right. intros E' HE'WF G' HG'WF.
+  (* program store *)
+  - right. intros E' HE'WF SplitWF HEE'match G'.
     exists (PLTT.PC (C1, PLTT.to_partial_stack d0 split,
                      Memory.set pmem C1
                                 (Register.get r1 regs1)
@@ -269,7 +149,7 @@ Proof.
                      regs1, pc1+1)).
     split.
     (* step *)
-    + destruct (PLTT.split_wellformed G' HG'WF C1 Hcontrol)
+    + destruct (PLTT.split_wellformed G' C1 Hcontrol)
         as [C1I [C1_in_Is C1I_name]].
       destruct (HmemWF C1I C1 C1_in_Is C1I_name)
         as [C1mem HC1mem].
@@ -287,7 +167,7 @@ Proof.
       * apply M.add_1. reflexivity.
       * unfold G'. simpl.
         unfold PLTT.maps_match_on.
-        intros. split; intro; apply HE'WF; assumption.
+        intros. split; intro; apply HEE'match; assumption.
       * simpl. 
         unfold G in Hstep.
         rewrite H5 in H. inversion H.
@@ -319,222 +199,63 @@ Proof.
           try assumption;
           reflexivity.
 
-  - right.
-    intros E' HE'WF G' HG'WF.
-    eexists. split.
-    (* step *)
-    + destruct (PLTT.split_wellformed G' HG'WF C1 Hcontrol)
-        as [C1I [C1_in_Is C1I_name]].
-      destruct (HmemWF C1I C1 C1_in_Is C1I_name)
-        as [C1mem HC1mem].
-      eapply PLTT.Program_Epsilon.
-      * apply HC1mem.
-      * apply HC1mem.
-      * simpl. unfold PLTT.maps_match_on.
-        intros. split; intro; apply HE'WF; assumption.
-      * simpl. rewrite H4 in H.
-        inversion H.
-        rewrite H2 in Hstep.
-        rewrite H3 in Hstep.
-        rewrite H5 in Hstep.
-        rewrite H6 in Hstep.
-        rewrite H7 in Hstep.
-        eapply Hstep.
-      * apply Hmem. assumption.
-        rewrite H4 in H.
-        inversion H.
-        rewrite <- H2. assumption.
-      * eassumption.
-    (* states match *)
-    + simpl. rewrite H4 in H.
-      inversion H.
-      rewrite <- H7.
-      apply program_control.
-      rewrite <- H2. assumption.
-      reflexivity.
-      simpl. unfold PLTT.maps_match_on.
-      intros. split; intro; assumption.
-
-  - right.
-    intros E' HE'WF G' HG'WF.
-    eexists. split.
-    (* step *)
-    + destruct (PLTT.split_wellformed G' HG'WF C1 Hcontrol)
-        as [C1I [C1_in_Is C1I_name]].
-      destruct (HmemWF C1I C1 C1_in_Is C1I_name)
-        as [C1mem HC1mem].
-      eapply PLTT.Program_Epsilon.
-      * apply HC1mem.
-      * apply HC1mem.
-      * simpl. unfold PLTT.maps_match_on.
-        intros. split; intro; apply HE'WF; assumption.
-      * simpl. rewrite H3 in H.
-        inversion H.
-        rewrite H2 in Hstep.
-        rewrite H4 in Hstep.
-        rewrite H5 in Hstep.
-        rewrite H6 in Hstep.
-        eapply Hstep.
-      * apply Hmem. assumption.
-        rewrite H3 in H.
-        inversion H.
-        rewrite <- H2. assumption.
-      * eassumption.
-    (* states match *)
-    + simpl. rewrite H3 in H.
-      inversion H.
-      (* NOTE here we don't rewrite *)
-      apply program_control.
-      rewrite <- H2. assumption.
-      reflexivity.
-      simpl. unfold PLTT.maps_match_on.
-      intros. split; intro; assumption.
-
-  - right.
-    intros E' HE'WF G' HG'WF.
-    eexists. split.
-    (* step *)
-    + destruct (PLTT.split_wellformed G' HG'WF C1 Hcontrol)
-        as [C1I [C1_in_Is C1I_name]].
-      destruct (HmemWF C1I C1 C1_in_Is C1I_name)
-        as [C1mem HC1mem].
-      eapply PLTT.Program_Epsilon.
-      * apply HC1mem.
-      * apply HC1mem.
-      * simpl. unfold PLTT.maps_match_on.
-        intros. split; intro; apply HE'WF; assumption.
-      * simpl. rewrite H3 in H.
-        inversion H.
-        rewrite H4 in Hstep.
-        rewrite H5 in Hstep.
-        rewrite H6 in Hstep.
-        rewrite H7 in Hstep.
-        rewrite H8 in Hstep.
-        eapply Hstep.
-      * apply Hmem. assumption.
-        rewrite H3 in H.
-        inversion H.
-        rewrite <- H4. assumption.
-      * eassumption.
-    (* states match *)
-    + simpl. rewrite H3 in H.
-      inversion H.
-      rewrite <- H7.
-      apply program_control.
-      rewrite <- H4. assumption.
-      reflexivity.
-      simpl. unfold PLTT.maps_match_on.
-      intros. split; intro; assumption.
-
-  - right.
-    intros E' HE'WF G' HG'WF.
-    eexists. split.
-    (* step *)
-    + destruct (PLTT.split_wellformed G' HG'WF C1 Hcontrol)
-        as [C1I [C1_in_Is C1I_name]].
-      destruct (HmemWF C1I C1 C1_in_Is C1I_name)
-        as [C1mem HC1mem].
-      eapply PLTT.Program_Epsilon.
-      * apply HC1mem.
-      * apply HC1mem.
-      * simpl. unfold PLTT.maps_match_on.
-        intros. split; intro; apply HE'WF; assumption.
-      * simpl. rewrite H3 in H.
-        inversion H.
-        rewrite H4 in Hstep.
-        rewrite H5 in Hstep.
-        rewrite H6 in Hstep.
-        rewrite H7 in Hstep.
-        rewrite H8 in Hstep.
-        eapply Hstep.
-      * apply Hmem. assumption.
-        rewrite H3 in H.
-        inversion H.
-        rewrite <- H4. assumption.
-      * eassumption.
-    (* states match *)
-    + simpl. rewrite H3 in H.
-      inversion H.
-      rewrite <- H7.
-      apply program_control.
-      rewrite <- H4. assumption.
-      reflexivity.
-      simpl. unfold PLTT.maps_match_on.
-      intros. split; intro; assumption.
-
   (* program is calling *)
   - right.
-    intros E' HE'WF G' HG'WF.
-    destruct (in_dec Nat.eq_dec C' split) as [ HC'origin | ? ].
-    (* internal call *)
-    + eexists. split.
-      (* step *)
-      * apply PLTT.Program_Internal_Call;
-          try assumption;
-          reflexivity.
-      (* states match *)
-      * unfold PLTT.maps_match_on in HE'WF.
-        destruct
-          (PLTT.split_wellformed G' HG'WF C' HC'origin)
-          as [CI HCI].
-        destruct HCI as [CI_in_Is CI_name_is_C'].
-        destruct (PLTT.entrypoints_exist
-                    G' HG'WF CI C' CI_in_Is CI_name_is_C')
-          as [C'_in_E' [addrs C'_mapsto_E']].
-        rewrite EntryPoint.get_works_locally with
-          (E':=E') (addrs:=addrs).
-        apply program_control;
-          try assumption.
-        ** simpl.
-           apply Util.in_implies_mem_true in Hcontrol.
-           rewrite Hcontrol.
-           reflexivity.
-        ** apply HE'WF. assumption. assumption.
-        ** assumption.
-    (* external call *)
-    + eexists. split.
-      (* step *)
-      * apply PLTT.Program_External_Call;
-          try assumption;
-          reflexivity.
-      (* states match *)
-      * apply context_control.
-        ** assumption.
-        ** simpl.
-           apply Util.in_implies_mem_true in Hcontrol.
-           rewrite Hcontrol.
-           reflexivity.
-        ** assumption.
+    intros E' HE'WF SplitWF HEE'match G'.
+    destruct (in_dec Nat.eq_dec C' split) as [ HC'origin | ? ];
+      eexists; split.
+    (* internal call - step *)
+    + apply PLTT.Program_Internal_Call; auto.
+    (* internal call - states match *)
+    + unfold PLTT.maps_match_on in HEE'match.
+      destruct (PLTT.split_wellformed G' C' HC'origin)
+        as [CI HCI].
+      destruct HCI as [CI_in_Is CI_name_is_C'].
+      destruct (PLTT.entrypoints_exist
+                  G' CI C' CI_in_Is CI_name_is_C')
+        as [C'_in_E' [addrs C'_mapsto_E']].
+      rewrite EntryPoint.get_works_locally with
+        (E':=E') (addrs:=addrs).
+      apply program_control;
+        try auto.
+      * simpl.
+        apply Util.in_implies_mem_true in Hcontrol.
+        rewrite Hcontrol.
+        reflexivity.
+      * apply HEE'match; auto.
+      * auto.
+    (* external call - step *)
+    + apply PLTT.Program_External_Call; auto.
+    (* external call - states match *)
+    + apply context_control;
+        try auto.
+      * simpl.
+        apply Util.in_implies_mem_true in Hcontrol.
+        rewrite Hcontrol.
+        reflexivity.
 
   (* program is returning *)
   - right.
-    intros E' HE'WF G' HG'WF.
+    intros E' HE'WF SplitWF HEE'match G'.
     destruct (in_dec Nat.eq_dec C' split)
-      as [ HC'origin | HC'origin ].
-    (* internal return *)
-    + eexists. split.
-      (* step *)
-      * apply PLTT.Program_Internal_Return;
-          try assumption.
-        ** simpl.
-           apply Util.in_implies_mem_true in HC'origin.
-           rewrite HC'origin. reflexivity.
-      (* states match *)
-      * apply program_control;
-          try assumption;
-          reflexivity.
-    (* external return *)
-    + eexists. split.
-      (* step *)
-      * apply PLTT.Program_External_Return;
-          try assumption.
-          ** simpl.
-             apply Util.not_in_implies_mem_false in HC'origin.
-             rewrite HC'origin. reflexivity.
-      (* states match *)
-      * apply context_control;
-          try assumption;
-          reflexivity.
+      as [ HC'origin | HC'origin ];
+      eexists; split.
+    (* internal return - step *)
+    + apply PLTT.Program_Internal_Return;
+        try auto.
+      * simpl.
+        apply Util.in_implies_mem_true in HC'origin.
+        rewrite HC'origin. reflexivity.
+    (* internal return - states match *)
+    + apply program_control; auto.
+    (* external return - step *)
+    + apply PLTT.Program_External_Return;
+        try auto.
+      * simpl.
+        apply Util.not_in_implies_mem_false in HC'origin.
+        rewrite HC'origin. reflexivity.
+    (* external return - states match *)
+    + apply context_control; auto.
 
   (* context store *)
   - unfold PLTT.maps_match_on.
@@ -542,7 +263,7 @@ Proof.
     split.
     + intro HC'map.
       apply Hmem.
-      * assumption.
+      * auto.
       * destruct (M.find (elt:=list nat) C1 mem1) eqn:HC1find.
         ** unfold Memory.set in HC'map.
            rewrite HC1find in HC'map.
@@ -564,13 +285,13 @@ Proof.
         ** assert (HC'mem: PLTT.M.MapsTo C' C'mem mem1).
            { apply Hmem; assumption. }
            eapply M.add_2; assumption.
-        ** apply Hmem; assumption.
+        ** apply Hmem; auto.
 
   (* context call is calling *) 
   - right.
     destruct (in_dec Nat.eq_dec C' split)
       as [ HC'origin | ? ];
-      intros E' HE'WF G' HG'WF; eexists; split.
+      intros E' HE'WF SplitWF HEE'match G'; eexists; split.
     (* external call - step *)
     + apply PLTT.Context_External_Call;
         try assumption.
@@ -578,19 +299,18 @@ Proof.
         eassumption.
         reflexivity.
     (* external call - states match *)
-    + unfold PLTT.maps_match_on in HE'WF.
-      destruct (PLTT.split_wellformed G' HG'WF C' HC'origin)
+    + unfold PLTT.maps_match_on in HEE'match.
+      destruct (PLTT.split_wellformed G' C' HC'origin)
         as [CI HCI].
       destruct HCI as [CI_in_Is CI_name_is_C'].
       destruct (PLTT.entrypoints_exist
-                  G' HG'WF CI C' CI_in_Is CI_name_is_C')
+                  G' CI C' CI_in_Is CI_name_is_C')
         as [C'_in_E' [addrs C'_mapsto_E']].
       rewrite EntryPoint.get_works_locally with
         (E':=E') (addrs:=addrs).
       apply program_control;
-        try assumption;
-        try reflexivity.
-      * apply (HE'WF C' addrs);
+        auto.
+      * apply (HEE'match C' addrs);
           assumption.
       * assumption.
 
@@ -601,14 +321,12 @@ Proof.
         eassumption.
         reflexivity.
     (* internal call - states match *)
-    + apply context_control;
-        try assumption;
-        reflexivity.
+    + apply context_control; auto.
 
   (* context is returning *)
   - right.
     destruct (in_dec Nat.eq_dec C' split) as [HC'origin | ?];
-      intros E' HE'WF G' HG'WF; eexists; split.
+      intros E' HE'WF SplitWF HEE'match G'; eexists; split.
     (* external return - step*)
     + apply PLTT.Context_External_Return.
       * simpl. apply Util.in_implies_mem_true in HC'origin.
@@ -616,17 +334,13 @@ Proof.
         reflexivity.
       * assumption.
     (* external return - states match *)
-    + apply program_control;
-        try assumption;
-        reflexivity.
+    + apply program_control; auto.
 
     (* internal return - step *)
     + apply PLTT.Context_Internal_Return.
       * intro HCeqC'. apply H3. symmetry. apply HCeqC'.
       * assumption.
-      * apply PLTT.push_by_context_preserves_partial_stack.
-        ** assumption.
-        ** reflexivity.
+      * apply PLTT.push_by_context_preserves_partial_stack; auto.
     (* internal return - states match *)
     + apply context_control;
         try assumption;
